@prefix rdf: <http://www.w3.org/1999/02/22-rdf-syntax-ns#> .
@prefix exif: <http://www.kanzaki.com/ns/exif#> .
@prefix nid3: <http://www.semanticdesktop.org/ontologies/2007/05/10/nid3#> .
@prefix nrl: <http://www.semanticdesktop.org/ontologies/2007/08/15/nrl#> .
@prefix nfo: <http://www.semanticdesktop.org/ontologies/2007/03/22/nfo#> .
@prefix xsd: <http://www.w3.org/2001/XMLSchema#> .
@prefix tmo: <http://www.semanticdesktop.org/ontologies/2008/05/20/tmo#> .
@prefix protege: <http://protege.stanford.edu/system#> .
@prefix nmo: <http://www.semanticdesktop.org/ontologies/2007/03/22/nmo#> .
@prefix rdfs: <http://www.w3.org/2000/01/rdf-schema#> .
@prefix nexif: <http://www.semanticdesktop.org/ontologies/2007/05/10/nexif#> .
@prefix ncal: <http://www.semanticdesktop.org/ontologies/2007/04/02/ncal#> .
@prefix pimo: <http://www.semanticdesktop.org/ontologies/2007/11/01/pimo#> .
@prefix dcterms: <http://purl.org/dc/terms/> .
@prefix nao: <http://www.semanticdesktop.org/ontologies/2007/08/15/nao#> .
@prefix geo: <http://www.w3.org/2003/01/geo/wgs84_pos#> .
@prefix dc: <http://purl.org/dc/elements/1.1/> .
@prefix nie: <http://www.semanticdesktop.org/ontologies/2007/01/19/nie#> .
@prefix nco: <http://www.semanticdesktop.org/ontologies/2007/03/22/nco#> .

<http://www.semanticdesktop.org/ontologies/2007/03/22/nco#>
    nao:creator <http://www.dfki.uni-kl.de/~mylka> ;
    nao:description "The Nepomuk Contact Ontology describes contact information, common in many places on the desktop. It evolved from the VCARD specification (RFC 2426) and has been inspired by the Vcard Ontology by Renato Ianella. The scope of NCO is much broader though." ;
    nao:hasDefaultNamespace "http://www.semanticdesktop.org/ontologies/2007/03/22/nco#" ;
    nao:hasDefaultNamespaceAbbreviation "nco" ;
    nao:lastModified "2011-12-13T12:44:58Z" ;
    nao:prefLabel "Nepomuk Contact Ontology" ;
    nao:status "Unstable" ;
    nao:updatable "0 " ;
    nao:version "${SHAREDDESKTOPONTOLOGIES_VERSION}" ;
    a nrl:Ontology .

nco:Affiliation
    a rdfs:Class ;
    rdfs:comment "Aggregates three properties defined in RFC2426. Originally all three were attached directly to a person. One person could have only one title and one role within one organization. This class is intended to lift this limitation." ;
    rdfs:label "Affiliation" ;
    rdfs:subClassOf nco:Role .

nco:AudioIMAccount
    nao:deprecated true ;
    a rdfs:Class ;
    rdfs:comment "Deprecated in favour of nco:imCapabilityAudio." ;
    rdfs:label "AudioIMAccount" ;
    rdfs:subClassOf nco:IMAccount .

nco:BbsNumber
    a rdfs:Class ;
    rdfs:comment "A Bulletin Board System (BBS) phone number. Inspired by the (TYPE=bbsl) parameter of the TEL property as defined in RFC 2426 sec  3.3.1." ;
    rdfs:label "BbsNumber" ;
    rdfs:subClassOf nco:ModemNumber .

nco:CarPhoneNumber
    a rdfs:Class ;
    rdfs:comment "A car phone number. Inspired by the (TYPE=car) parameter of the TEL property as defined in RFC 2426 sec  3.3.1." ;
    rdfs:label "CarPhoneNumber" ;
    rdfs:subClassOf nco:VoicePhoneNumber .

nco:CellPhoneNumber
    a rdfs:Class ;
    rdfs:comment "A cellular phone number. Inspired by the (TYPE=cell) parameter of the TEL property as defined in RFC 2426 sec  3.3.1. Usually a cellular phone can accept voice calls as well as textual messages (SMS), therefore this class has two superclasses." ;
    rdfs:label "CellPhoneNumber" ;
    rdfs:subClassOf nco:MessagingNumber, nco:VoicePhoneNumber .

nco:Contact
    a rdfs:Class ;
    rdfs:comment "A Contact. A piece of data that can provide means to identify or communicate with an entity." ;
    rdfs:label "Contact" ;
    rdfs:subClassOf nie:InformationElement, nco:Role, nao:Party .

nco:ContactGroup
    a rdfs:Class ;
    rdfs:comment "A group of Contacts. Could be used to express a group in an addressbook or on a contact list of an IM application. One contact can belong to many groups." ;
    rdfs:label "ContactGroup" ;
    rdfs:subClassOf nie:InformationElement .

nco:ContactList
    a rdfs:Class ;
    rdfs:comment "A contact list, this class represents an addressbook or a contact list of an IM application. Contacts inside a contact list can belong to contact groups." ;
    rdfs:label "ContactList" ;
    rdfs:subClassOf nie:InformationElement .

nco:ContactListDataObject
    a rdfs:Class ;
    rdfs:comment "An entity occuring on a contact list (usually interpreted as an nco:Contact)" ;
    rdfs:label "ContactListDataObject" ;
    rdfs:subClassOf nie:DataObject .

nco:ContactMedium
    a rdfs:Class ;
    rdfs:comment "A superclass for all contact media - ways to contact an entity represented by a Contact instance. Some of the subclasses of this class (the various kinds of telephone numbers and postal addresses) have been inspired by the values of the TYPE parameter of ADR and TEL properties defined in RFC 2426 sec. 3.2.1. and 3.3.1 respectively. Each value is represented by an appropriate subclass with two major exceptions TYPE=home and TYPE=work. They are to be expressed by the roles these contact media are attached to i.e. contact media with TYPE=home parameter are to be attached to the default role (nco:Contact or nco:PersonContact), whereas media with TYPE=work parameter should be attached to nco:Affiliation or nco:OrganizationContact." ;
    rdfs:label "ContactMedium" ;
    rdfs:subClassOf rdfs:Resource .

nco:DomesticDeliveryAddress
    a rdfs:Class ;
    rdfs:comment "Domestic Delivery Addresse. Class inspired by TYPE=dom parameter of the ADR property defined in RFC 2426 sec. 3.2.1" ;
    rdfs:label "DomesticDeliveryAddress" ;
    rdfs:subClassOf nco:PostalAddress .

nco:EmailAddress
    a rdfs:Class ;
    rdfs:comment "An email address. The recommended best practice is to use mailto: uris for instances of this class." ;
    rdfs:label "EmailAddress" ;
    rdfs:subClassOf nco:ContactMedium .

nco:FaxNumber
    a rdfs:Class ;
    rdfs:comment "A fax number. Inspired by the (TYPE=fax) parameter of the TEL property as defined in RFC 2426 sec  3.3.1." ;
    rdfs:label "FaxNumber" ;
    rdfs:subClassOf nco:PhoneNumber .

nco:Gender
    a rdfs:Class ;
    rdfs:comment "Gender. Instances of this class may include male and female." ;
    rdfs:label "Gender" ;
    rdfs:subClassOf rdfs:Resource .

nco:IMAccount
    a rdfs:Class ;
    rdfs:comment "An account in an Instant Messaging system." ;
    rdfs:label "IMAccount" ;
    rdfs:subClassOf nco:ContactMedium .

nco:IMCapability
    a rdfs:Class ;
    rdfs:comment "Capabilities of a cetain IMAccount." ;
    rdfs:label "imCapability" ;
    rdfs:subClassOf rdfs:Resource .

nco:IMStatusType
    a rdfs:Class ;
    rdfs:comment "The status type of an IMAccount. Based on the Connection_Presence_Type enumeration of the Telepathy project: http://telepathy.freedesktop.org/spec/Connection_Interface_Simple_Presence.html#Enum:Connection_Presence_Type" ;
    rdfs:label "instant messaging status type" ;
    rdfs:subClassOf rdfs:Resource .

nco:IMStatusTypeAvailable
    a nco:IMStatusType ;
    rdfs:label "available" .

nco:IMStatusTypeAway
    a nco:IMStatusType ;
    rdfs:label "away" .

nco:IMStatusTypeBusy
    a nco:IMStatusType ;
    rdfs:label "busy" .

nco:IMStatusTypeExtendedAway
    a nco:IMStatusType ;
    rdfs:label "extended away" .

nco:IMStatusTypeHidden
    a nco:IMStatusType ;
    rdfs:label "hidden" .

nco:IMStatusTypeOffline
    a nco:IMStatusType ;
    rdfs:label "offline" .

nco:IMStatusTypeUnknown
    a nco:IMStatusType ;
    rdfs:label "unknown" .

nco:InternationalDeliveryAddress
    a rdfs:Class ;
    rdfs:comment "International Delivery Addresse. Class inspired by TYPE=intl parameter of the ADR property defined in RFC 2426 sec. 3.2.1" ;
    rdfs:label "InternationalDeliveryAddress" ;
    rdfs:subClassOf nco:PostalAddress .

nco:IsdnNumber
    a rdfs:Class ;
    rdfs:comment "An ISDN phone number. Inspired by the (TYPE=isdn) parameter of the TEL property as defined in RFC 2426 sec  3.3.1." ;
    rdfs:label "IsdnNumber" ;
    rdfs:subClassOf nco:VoicePhoneNumber .

nco:MessagingNumber
    a rdfs:Class ;
    rdfs:comment "A number that can accept textual messages." ;
    rdfs:label "MessagingNumber" ;
    rdfs:subClassOf nco:PhoneNumber .

nco:ModemNumber
    a rdfs:Class ;
    rdfs:comment "A modem phone number. Inspired by the (TYPE=modem) parameter of the TEL property as defined in RFC 2426 sec  3.3.1." ;
    rdfs:label "ModemNumber" ;
    rdfs:subClassOf nco:PhoneNumber .

nco:OrganizationContact
    a rdfs:Class ;
    rdfs:comment "A Contact that denotes on Organization." ;
    rdfs:label "OrganizationContact" ;
    rdfs:subClassOf nco:Contact .

nco:PagerNumber
    a rdfs:Class ;
    rdfs:comment "A pager phone number. Inspired by the (TYPE=pager) parameter of the TEL property as defined in RFC 2426 sec  3.3.1." ;
    rdfs:label "PagerNumber" ;
    rdfs:subClassOf nco:MessagingNumber .

nco:ParcelDeliveryAddress
    a rdfs:Class ;
    rdfs:comment "Parcel Delivery Addresse. Class inspired by TYPE=parcel parameter of the ADR property defined in RFC 2426 sec. 3.2.1" ;
    rdfs:label "ParcelDeliveryAddress" ;
    rdfs:subClassOf nco:PostalAddress .

nco:PcsNumber
    a rdfs:Class ;
    rdfs:comment "Personal Communication Services Number. A class inspired by the TYPE=pcs parameter of the TEL property defined in RFC 2426 sec. 3.3.1" ;
    rdfs:label "PcsNumber" ;
    rdfs:subClassOf nco:VoicePhoneNumber .

nco:PersonContact
    a rdfs:Class ;
    rdfs:comment "A Contact that denotes a Person. A person can have multiple Affiliations." ;
    rdfs:label "PersonContact" ;
    rdfs:subClassOf nco:Contact .

nco:PhoneNumber
    a rdfs:Class ;
    rdfs:comment "A telephone number." ;
    rdfs:label "PhoneNumber" ;
    rdfs:subClassOf nco:ContactMedium .

nco:PostalAddress
    a rdfs:Class ;
    rdfs:comment "A postal address. A class aggregating the various parts of a value for the 'ADR' property as defined in RFC 2426 Sec. 3.2.1." ;
    rdfs:label "PostalAddress" ;
    rdfs:subClassOf nco:ContactMedium .

nco:Role
    a rdfs:Class ;
    rdfs:comment "A role played by a contact. Contacts that denote people, can have many roles (e.g. see the hasAffiliation property and Affiliation class). Contacts that denote Organizations or other Agents usually have one role.  Each role can introduce additional contact media." ;
    rdfs:label "Role" ;
    rdfs:subClassOf rdfs:Resource .

nco:VideoIMAccount
    nao:deprecated true ;
    a rdfs:Class ;
    rdfs:comment "Deprecated in favour of nco:imCapabilityVideo." ;
    rdfs:label "VideoIMAccount" ;
    rdfs:subClassOf nco:AudioIMAccount .

nco:VideoTelephoneNumber
    a rdfs:Class ;
    rdfs:comment "A Video telephone number. A class inspired by the TYPE=video parameter of the TEL property defined in RFC 2426 sec. 3.3.1" ;
    rdfs:label "VideoTelephoneNumber" ;
    rdfs:subClassOf nco:VoicePhoneNumber .

nco:VoicePhoneNumber
    a rdfs:Class ;
    rdfs:comment "A telephone number with voice communication capabilities. Class inspired by the TYPE=voice parameter of the TEL property defined in RFC 2426 sec. 3.3.1" ;
    rdfs:label "VoicePhoneNumber" ;
    rdfs:subClassOf nco:PhoneNumber .

nco:addressLocation
    nrl:maxCardinality "1" ;
    a nrl:DefiningProperty, rdf:Property ;
    rdfs:comment "The geographical location of a postal address." ;
    rdfs:domain nco:PostalAddress ;
    rdfs:label "addressLocation" ;
    rdfs:range geo:Point .

nco:belongsToGroup
    a rdf:Property ;
    rdfs:comment "Links a Contact with a ContactGroup it belongs to." ;
    rdfs:domain nco:Contact ;
    rdfs:label "belongsToGroup" ;
    rdfs:range nco:ContactGroup .

nco:birthDate
    nrl:maxCardinality 1 ;
    a rdf:Property ;
    rdfs:comment "Birth date of the object represented by this Contact. An equivalent of the 'BDAY' property as defined in RFC 2426 Sec. 3.1.5." ;
    rdfs:domain nco:Contact ;
    rdfs:label "birthDate" ;
    rdfs:range xsd:date ;
    rdfs:subPropertyOf dc:date .

nco:blogUrl
    a nrl:DefiningProperty, rdf:Property ;
    rdfs:comment "A Blog url." ;
    rdfs:domain nco:Role ;
    rdfs:label "blogUrl" ;
    rdfs:range rdfs:Resource ;
    rdfs:subPropertyOf nco:url .

nco:contactGroupName
    nrl:maxCardinality 1 ;
    a rdf:Property ;
    rdfs:comment """The name of the contact group. This property was NOT defined 
    in the VCARD standard. See documentation of the 'ContactGroup' class for 
    details""" ;
    rdfs:domain nco:ContactGroup ;
    rdfs:label "contactGroupName" ;
    rdfs:range xsd:string ;
    rdfs:subPropertyOf dc:title .

nco:contactMediumComment
    nao:deprecated true ;
    a rdf:Property ;
    rdfs:comment "A comment about the contact medium. (Deprecated in favor of nie:comment or nao:description - based on the context)" ;
    rdfs:domain nco:ContactMedium ;
    rdfs:label "contactMediumComment" ;
    rdfs:range xsd:string .

nco:contactUID
    nrl:maxCardinality "1" ;
    a rdf:Property ;
    rdfs:comment "A value that represents a globally unique  identifier corresponding to the individual or resource associated with the Contact. An equivalent of the 'UID' property defined in RFC 2426 Sec. 3.6.7" ;
    rdfs:domain nco:Contact ;
    rdfs:label "contactUID" ;
    rdfs:range xsd:string ;
    rdfs:subPropertyOf nie:identifier .

nco:containsContact
    a nrl:DefiningProperty, rdf:Property ;
    rdfs:comment """A property used to group contacts into contact groups. This 
    property was NOT defined in the VCARD standard. See documentation for the 
    'ContactList' class for details""" ;
    rdfs:domain nco:ContactList ;
    rdfs:label "containsContact" ;
    rdfs:range nco:ContactListDataObject ;
    rdfs:subPropertyOf nie:hasPart .

nco:contributor
    a nrl:DefiningProperty, rdf:Property ;
    rdfs:comment "An entity responsible for making contributions to the content of the InformationElement." ;
    rdfs:domain nie:InformationElement ;
    rdfs:label "contributor" ;
    rdfs:range nco:Contact ;
    rdfs:subPropertyOf dc:contributor, nao:contributor .

nco:country
    nrl:maxCardinality 1 ;
    a rdf:Property ;
    rdfs:comment "A part of an address specyfing the country. Inspired by the seventh part of the value of the 'ADR' property as defined in RFC 2426, sec. 3.2.1" ;
    rdfs:domain nco:PostalAddress ;
    rdfs:label "country" ;
    rdfs:range xsd:string .

nco:creator
    a nrl:DefiningProperty, rdf:Property ;
    rdfs:comment "Creator of an information element, an entity primarily responsible for the creation of the content of the data object." ;
    rdfs:domain nie:InformationElement ;
    rdfs:label "creator" ;
    rdfs:range nco:Contact ;
    rdfs:subPropertyOf dc:creator, nco:contributor, nao:creator .

nco:department
    a rdf:Property ;
    rdfs:comment "Department. The organizational unit within the organization." ;
    rdfs:domain nco:Affiliation ;
    rdfs:label "department" ;
    rdfs:range xsd:string .

nco:emailAddress
    nrl:maxCardinality 1 ;
    a rdf:Property ;
    rdfs:domain nco:EmailAddress ;
    rdfs:label "emailAddress" ;
    rdfs:range xsd:string ;
    rdfs:subPropertyOf nao:identifier .

nco:end
    nrl:maxCardinality 1 ;
    a rdf:Property ;
    rdfs:comment "End datetime for the role, such as: the datetime of leaving a project or organization, datetime of ending employment, datetime of divorce. If absent or set to a date in the future, the role is currently active." ;
    rdfs:domain nco:Role ;
    rdfs:label "end" ;
    rdfs:range xsd:dateTime .

nco:extendedAddress
    nrl:maxCardinality "1" ;
    a rdf:Property ;
    rdfs:comment "An extended part of an address. This field might be used to express parts of an address that aren't include in the name of the Contact but also aren't part of the actual location. Usually the streed address and following fields are enough for a postal letter to arrive. Examples may include ('University of California Campus building 45', 'Sears Tower 34th floor' etc.) Inspired by the second part of the value of the 'ADR' property as defined in RFC 2426, sec. 3.2.1" ;
    rdfs:domain nco:PostalAddress ;
    rdfs:label "extendedAddress" ;
    rdfs:range xsd:string .

nco:female
    a nco:Gender ;
    rdfs:comment "A Female" ;
    rdfs:label "female" .

nco:foafUrl
    a rdf:Property ;
    rdfs:comment "The URL of the FOAF file." ;
    rdfs:domain nco:Role ;
    rdfs:label "foafUrl" ;
    rdfs:range rdfs:Resource ;
    rdfs:subPropertyOf nco:url .

nco:fullname
    nrl:maxCardinality "1" ;
    a rdf:Property ;
    rdfs:comment "To specify the formatted text corresponding to the name of the object the Contact represents. An equivalent of the FN property as defined in RFC 2426 Sec. 3.1.1." ;
    rdfs:domain nco:Contact ;
    rdfs:label "fullname" ;
    rdfs:range xsd:string ;
    rdfs:subPropertyOf nie:title .

nco:gender
    nrl:maxCardinality 1 ;
    a rdf:Property ;
    rdfs:comment "Gender of the given contact." ;
    rdfs:domain nco:PersonContact ;
    rdfs:label "gender" ;
    rdfs:range nco:Gender .

nco:hasAffiliation
    a nrl:DefiningProperty, rdf:Property ;
    rdfs:comment "Links a PersonContact with an Affiliation." ;
    rdfs:domain nco:PersonContact ;
    rdfs:label "hasAffiliation" ;
    rdfs:range nco:Affiliation .

nco:hasContactMedium
    a nrl:DefiningProperty, rdf:Property ;
    rdfs:comment "A superProperty for all properties linking a Contact to an instance of a contact medium." ;
    rdfs:domain nco:Role ;
    rdfs:label "hasContactMedium" ;
    rdfs:range nco:ContactMedium .

nco:hasEmailAddress
    a rdf:Property ;
    rdfs:comment "An address for electronic mail communication with the object specified by this contact. An equivalent of the 'EMAIL' property as defined in RFC 2426 Sec. 3.3.1." ;
    rdfs:domain nco:Role ;
    rdfs:label "hasEmailAddress" ;
    rdfs:range nco:EmailAddress ;
    rdfs:subPropertyOf nco:hasContactMedium .

nco:hasIMAccount
    a rdf:Property ;
    rdfs:comment "Indicates that an Instant Messaging account owned by an entity represented by this contact." ;
    rdfs:domain nco:Role ;
    rdfs:label "hasIMAccount" ;
    rdfs:range nco:IMAccount ;
    rdfs:subPropertyOf nco:hasContactMedium .

nco:hasIMCapability
    a nrl:DefiningProperty, rdf:Property ;
    rdfs:comment "Indicates that an IMAccount has a certain capability." ;
    rdfs:domain nco:IMAccount ;
    rdfs:label "hasIMCapability" ;
    rdfs:range nco:IMCapability .

nco:hasLocation
    nrl:maxCardinality "1" ;
    a rdf:Property ;
    rdfs:comment "Geographical location of the contact. Inspired by the 'GEO' property specified in RFC 2426 Sec. 3.4.2" ;
    rdfs:domain nco:Contact ;
    rdfs:label "hasLocation" ;
    rdfs:range geo:Point .

nco:hasPhoneNumber
    a rdf:Property ;
    rdfs:comment "A number for telephony communication with the object represented by this Contact. An equivalent of the 'TEL' property defined in RFC 2426 Sec. 3.3.1" ;
    rdfs:domain nco:Role ;
    rdfs:label "hasPhoneNumber" ;
    rdfs:range nco:PhoneNumber ;
    rdfs:subPropertyOf nco:hasContactMedium .

nco:hasPostalAddress
    a rdf:Property ;
    rdfs:comment "The default Address for a Contact. An equivalent of the 'ADR' property as defined in RFC 2426 Sec. 3.2.1." ;
    rdfs:domain nco:Role ;
    rdfs:label "hasPostalAddress" ;
    rdfs:range nco:PostalAddress ;
    rdfs:subPropertyOf nco:hasContactMedium .

nco:hobby
    a rdf:Property ;
    rdfs:comment "A hobby associated with a PersonContact. This property can be used to express hobbies and interests." ;
    rdfs:domain nco:PersonContact ;
    rdfs:label "hobby" ;
    rdfs:range xsd:string .

nco:imAccountType
    nrl:maxCardinality "1" ;
    a rdf:Property ;
    rdfs:comment "Type of the IM account. This may be the name of the service that provides the IM functionality. Examples might include Jabber, ICQ, MSN etc" ;
    rdfs:domain nco:IMAccount ;
    rdfs:label "imAccountType" ;
    rdfs:range xsd:string .

nco:imCapabilityAudio
    a nco:IMCapability .

nco:imCapabilityText
    a nco:IMCapability .

nco:imCapabilityVideo
    a nco:IMCapability .

nco:imID
    a rdf:Property ;
    rdfs:comment "Identifier of the IM account. Examples of such identifier might include ICQ UINs, Jabber IDs, Skype names etc." ;
    rdfs:domain nco:IMAccount ;
    rdfs:label "imID" ;
    rdfs:range xsd:string ;
    rdfs:subPropertyOf nao:identifier .

nco:imNickname
    a rdf:Property ;
    rdfs:comment "A nickname attached to a particular IM Account." ;
    rdfs:domain nco:IMAccount ;
    rdfs:label "imNickname" ;
    rdfs:range xsd:string .

nco:imStatus
    nrl:maxCardinality 1 ;
    a nrl:NonDefiningProperty, rdf:Property ;
    rdfs:comment "Current status of the given IM account. When this property is set, the nco:imStatusType should also always be set. Applications should attempt to parse this property to determine the presence, only falling back to the nco:imStatusType property in the case that this property's value is unrecognised. Values for this property may include 'available', 'offline', 'busy' etc. The exact choice of them is unspecified, although it is recommended to follow the guidance of the Telepathy project when choosing a string identifier http://telepathy.freedesktop.org/spec/Connection_Interface_Simple_Presence.html#description" ;
    rdfs:domain nco:IMAccount ;
    rdfs:label "imStatus" ;
    rdfs:range xsd:string .

nco:imStatusMessage
    nrl:maxCardinality "1" ;
    a nrl:NonDefiningProperty, rdf:Property ;
    rdfs:comment "A feature common in most IM systems. A message left by the user for all his/her contacts to see." ;
    rdfs:domain nco:IMAccount ;
    rdfs:label "imStatusMessage" ;
    rdfs:range xsd:string .

nco:imStatusType
    nrl:maxCardinality 1 ;
    a rdf:Property ;
    rdfs:comment "Current status type of the given IM account. When this property is set, the nco:imStatus property should also always be set. Applications should attempt to parse the nco:imStatus property to determine the presence, only falling back to this property in the case that the nco:imStatus property's value is unrecognised." ;
    rdfs:domain nco:IMAccount ;
    rdfs:label "instant messaging status type" ;
    rdfs:range nco:IMStatusType .

nco:isAccessedBy
    a rdf:Property ;
    rdfs:comment "Indicates the local IMAccount by which this IMAccount is accessed. This does not imply membership of a contact list." ;
    rdfs:domain nco:IMAccount ;
    rdfs:label "isKnownBy" ;
    rdfs:range nco:IMAccount .

nco:isBlocked
    nrl:maxCardinality "1" ;
    a rdf:Property ;
    rdfs:comment "Indicates that this IMAccount has been blocked." ;
    rdfs:domain nco:IMAccount ;
    rdfs:label "isBlocked" ;
    rdfs:range xsd:boolean .

nco:key
    a rdf:Property ;
    rdfs:comment "An encryption key attached to a contact. Inspired by the KEY property defined in RFC 2426 sec. 3.7.2" ;
    rdfs:domain nco:Contact ;
    rdfs:label "key" ;
    rdfs:range nie:DataObject ;
    rdfs:subPropertyOf nie:hasPart .

nco:locality
    nrl:maxCardinality 1 ;
    a rdf:Property ;
    rdfs:comment "Locality or City. Inspired by the fourth part of the value of the 'ADR' property as defined in RFC 2426, sec. 3.2.1" ;
    rdfs:domain nco:PostalAddress ;
    rdfs:label "locality" ;
    rdfs:range xsd:string .

nco:logo
    a rdf:Property ;
    rdfs:comment "Logo of a company. Inspired by the LOGO property defined in RFC 2426 sec. 3.5.3" ;
    rdfs:domain nco:OrganizationContact ;
    rdfs:label "logo" ;
    rdfs:range nie:DataObject ;
    rdfs:subPropertyOf nie:hasPart .

nco:male
    a nco:Gender ;
    rdfs:comment "A Male" ;
    rdfs:label "male" .

nco:nameAdditional
    a rdf:Property ;
    rdfs:comment "Additional given name of an object represented by this contact. See documentation for 'nameFamily' property for details." ;
    rdfs:domain nco:PersonContact ;
    rdfs:label "nameAdditional" ;
    rdfs:range xsd:string .

nco:nameFamily
    nrl:maxCardinality "1" ;
    a rdf:Property ;
    rdfs:comment "The family name of an Object represented by this Contact. These applies to people that have more than one given name. The 'first' one is considered 'the' given name (see nameGiven) property. All additional ones are considered 'additional' names. The name inherited from parents is the 'family name'. e.g. For Dr. John Phil Paul Stevenson Jr. M.D. A.C.P. we have contact with: honorificPrefix: 'Dr.', nameGiven: 'John', nameAdditional: 'Phil', nameAdditional: 'Paul', nameFamily: 'Stevenson', honorificSuffix: 'Jr.', honorificSuffix: 'M.D.', honorificSuffix: 'A.C.P.'. These properties form an equivalent of the compound 'N' property as defined in RFC 2426 Sec. 3.1.2" ;
    rdfs:domain nco:PersonContact ;
    rdfs:label "nameFamily" ;
    rdfs:range xsd:string .

nco:nameGiven
    nrl:maxCardinality "1" ;
    a rdf:Property ;
    rdfs:comment "The given name for the object represented by this Contact. See documentation for 'nameFamily' property for details." ;
    rdfs:domain nco:PersonContact ;
    rdfs:label "nameGiven" ;
    rdfs:range xsd:string .

nco:nameHonorificPrefix
    a rdf:Property ;
    rdfs:comment "A prefix for the name of the object represented by this Contact. See documentation for the 'nameFamily' property for details." ;
    rdfs:domain nco:PersonContact ;
    rdfs:label "nameHonorificPrefix" ;
    rdfs:range xsd:string .

nco:nameHonorificSuffix
    a rdf:Property ;
    rdfs:comment "A suffix for the name of the Object represented by the given object. See documentation for the 'nameFamily' for details." ;
    rdfs:domain nco:PersonContact ;
    rdfs:label "nameHonorificSuffix" ;
    rdfs:range xsd:string .

nco:nickname
    a rdf:Property ;
    rdfs:comment "A nickname of the Object represented by this Contact. This is an equivalent of the 'NICKNAME' property as defined in RFC 2426 Sec. 3.1.3." ;
    rdfs:domain nco:Contact ;
    rdfs:label "nickname" ;
    rdfs:range xsd:string .

nco:note
    a rdf:Property ;
    rdfs:comment "A note about the object represented by this Contact. An equivalent for the 'NOTE' property defined in RFC 2426 Sec. 3.6.2" ;
    rdfs:domain nco:Contact ;
    rdfs:label "note" ;
    rdfs:range xsd:string ;
    rdfs:subPropertyOf nie:description .

nco:org
    nrl:maxCardinality "1" ;
    a nrl:DefiningProperty, rdf:Property ;
    rdfs:comment "Name of an organization or a unit within an organization the object represented by a Contact is associated with. An equivalent of the 'ORG' property defined in RFC 2426 Sec. 3.5.5" ;
    rdfs:domain nco:Affiliation ;
    rdfs:label "org" ;
    rdfs:range nco:OrganizationContact .

nco:phoneNumber
    nrl:maxCardinality "1" ;
    a rdf:Property ;
    rdfs:domain nco:PhoneNumber ;
    rdfs:label "phoneNumber" ;
    rdfs:range xsd:string .

nco:photo
    a rdf:Property ;
    rdfs:comment "Photograph attached to a Contact. The DataObject referred to by this property is usually interpreted as an nfo:Image. Inspired by the PHOTO property defined in RFC 2426 sec. 3.1.4" ;
    rdfs:domain nco:Contact ;
    rdfs:label "photo" ;
    rdfs:range nie:DataObject ;
    rdfs:subPropertyOf nie:hasPart .

nco:pobox
    nrl:maxCardinality "1" ;
    a rdf:Property ;
    rdfs:comment "Post office box. This is the first part of the value of the 'ADR' property as defined in RFC 2426, sec. 3.2.1" ;
    rdfs:domain nco:PostalAddress ;
    rdfs:label "pobox" ;
    rdfs:range xsd:string .

nco:postalcode
    nrl:maxCardinality 1 ;
    a rdf:Property ;
    rdfs:comment "Postal Code. Inspired by the sixth part of the value of the 'ADR' property as defined in RFC 2426, sec. 3.2.1" ;
    rdfs:domain nco:PostalAddress ;
    rdfs:label "postalcode" ;
    rdfs:range xsd:string .

nco:publisher
    a nrl:DefiningProperty, rdf:Property ;
    rdfs:comment "An entity responsible for making the InformationElement available." ;
    rdfs:domain nie:InformationElement ;
    rdfs:label "publisher" ;
    rdfs:range nco:Contact ;
    rdfs:subPropertyOf dc:publisher .

nco:publishesPresenceTo
    a rdf:Property ;
    rdfs:comment "Indicates that this IMAccount publishes its presence information to the other IMAccount." ;
    rdfs:domain nco:IMAccount ;
    rdfs:label "publishesPresenceTo" ;
    rdfs:range nco:IMAccount .

nco:region
    nrl:maxCardinality 1 ;
    a rdf:Property ;
    rdfs:comment "Region. Inspired by the fifth part of the value of the 'ADR' property as defined in RFC 2426, sec. 3.2.1" ;
    rdfs:domain nco:PostalAddress ;
    rdfs:label "region" ;
    rdfs:range xsd:string .

nco:representative
    a nrl:DefiningProperty, rdf:Property ;
    rdfs:comment "An object that represent an object represented by this Contact. Usually this property is used to link a Contact to an organization, to a contact to the representative of this organization the user directly interacts with. An equivalent for the 'AGENT' property defined in RFC 2426 Sec. 3.5.4" ;
    rdfs:domain nco:Contact ;
    rdfs:label "representative" ;
    rdfs:range nco:Contact .

nco:requestedPresenceSubscriptionTo
    a rdf:Property ;
    rdfs:comment "Indicates that this IMAccount has requested a subscription to the presence information of the other IMAccount." ;
    rdfs:domain nco:IMAccount ;
    rdfs:label "requestedPresenceSubscriptionTo" ;
    rdfs:range nco:IMAccount .

nco:role
    a rdf:Property ;
    rdfs:comment "Role an object represented by this contact represents in the organization. This might include 'Programmer', 'Manager', 'Sales Representative'. Be careful to avoid confusion with the title property. An equivalent of the 'ROLE' property as defined in RFC 2426. Sec. 3.5.2. Note the difference between nco:Role class and nco:role property." ;
    rdfs:domain nco:Affiliation ;
    rdfs:label "role" ;
    rdfs:range xsd:string .

nco:sound
    a rdf:Property ;
    rdfs:comment "Sound clip attached to a Contact. The DataObject referred to by this property is usually interpreted as an nfo:Audio. Inspired by the SOUND property defined in RFC 2425 sec. 3.6.6." ;
    rdfs:domain nco:Contact ;
    rdfs:label "sound" ;
    rdfs:range nie:DataObject ;
    rdfs:subPropertyOf nie:hasPart .

nco:start
    nrl:maxCardinality 1 ;
    a rdf:Property ;
    rdfs:comment "Start datetime for the role, such as: the datetime of joining a project or organization, datetime of starting employment, datetime of marriage" ;
    rdfs:domain nco:Role ;
    rdfs:label "start" ;
    rdfs:range xsd:dateTime .

nco:streetAddress
    nrl:maxCardinality "1" ;
    a rdf:Property ;
    rdfs:comment "The streed address. Inspired by the third part of the value of the 'ADR' property as defined in RFC 2426, sec. 3.2.1" ;
    rdfs:domain nco:PostalAddress ;
    rdfs:label "streetAddress" ;
    rdfs:range xsd:string .

nco:title
    nrl:maxCardinality "1" ;
    a rdf:Property ;
    rdfs:comment "The official title  the object represented by this contact in an organization. E.g. 'CEO', 'Director, Research and Development', 'Junior Software Developer/Analyst' etc. An equivalent of the 'TITLE' property defined in RFC 2426 Sec. 3.5.1" ;
    rdfs:domain nco:Affiliation ;
    rdfs:label "title" ;
    rdfs:range xsd:string .

nco:url
    a nrl:DefiningProperty, rdf:Property ;
    rdfs:comment "A uniform resource locator associated with the given role of a Contact. Inspired by the 'URL' property defined in RFC 2426 Sec. 3.6.8." ;
    rdfs:domain nco:Role ;
    rdfs:label "url" ;
    rdfs:range rdfs:Resource .

nco:voiceMail
    nrl:maxCardinality "1" ;
    a rdf:Property ;
    rdfs:comment "Indicates if the given number accepts voice mail. (e.g. there is an answering machine). Inspired by TYPE=msg parameter of the TEL property defined in RFC 2426 sec. 3.3.1" ;
    rdfs:domain nco:VoicePhoneNumber ;
    rdfs:label "voiceMail" ;
    rdfs:range xsd:boolean .

nco:websiteUrl
    a rdf:Property ;
    rdfs:comment "A url of a website." ;
    rdfs:domain nco:Role ;
    rdfs:label "websiteUrl" ;
    rdfs:range rdfs:Resource ;
    rdfs:subPropertyOf nco:url .

<http://www.semanticdesktop.org/ontologies/2007/03/22/nco_metadata#>
    nrl:coreGraphMetadataFor <http://www.semanticdesktop.org/ontologies/2007/03/22/nco#> ;
    a nrl:GraphMetadata .

