@prefix rdf: <http://www.w3.org/1999/02/22-rdf-syntax-ns#> .
@prefix rdfs: <http://www.w3.org/2000/01/rdf-schema#> .
@prefix ndo: <http://www.semanticdesktop.org/ontologies/2010/04/30/ndo#> .
@prefix nrl: <http://www.semanticdesktop.org/ontologies/2007/08/15/nrl#> .
@prefix nuao: <http://www.semanticdesktop.org/ontologies/2010/01/25/nuao#> .
@prefix nao: <http://www.semanticdesktop.org/ontologies/2007/08/15/nao#> .
@prefix nmo: <http://www.semanticdesktop.org/ontologies/2007/03/22/nmo#> .
@prefix nco: <http://www.semanticdesktop.org/ontologies/2007/03/22/nco#> .
@prefix xsd: <http://www.w3.org/2001/XMLSchema#> .
@prefix nie: <http://www.semanticdesktop.org/ontologies/2007/01/19/nie#> .
@prefix nfo: <http://www.semanticdesktop.org/ontologies/2007/03/22/nfo#> .

<http://www.semanticdesktop.org/ontologies/2010/04/30/ndo#>
    nao:description "The Nepomuk Download Ontology provides classes and properties to describe file downloads." ;
    nao:hasDefaultNamespace "http://www.semanticdesktop.org/ontologies/2010/04/30/ndo#" ;
    nao:hasDefaultNamespaceAbbreviation "ndo" ;
    nao:lastModified "2010-04-30T09:38:49Z" ;
    nao:prefLabel "Nepomuk Download Ontology " ;
    nao:serializationLanguage "TriG" ;
    nao:status "Testing" ;
    nao:version "${SHAREDDESKTOPONTOLOGIES_VERSION}" ;
    nrl:updatable "0" ;
    a nrl:DocumentGraph, nrl:KnowledgeBase .

ndo:DownloadEvent
    a rdfs:Class ;
    rdfs:comment "A single event (from the point of view of the user) of downloading of a file or a set of files. Use nuao:involves to indicate the files involved. The event is assigned to downloaded copies of files. Can be assigned to multiple files." ;
    rdfs:label "download event" ;
    rdfs:subClassOf nuao:DesktopEvent .

ndo:P2PFile
    a rdfs:Class ;
    rdfs:comment "A file available via a peer-to-peer network" ;
    rdfs:label "P2P file" ;
    rdfs:subClassOf nfo:RemoteDataObject .

ndo:Torrent
    a rdfs:Class ;
    rdfs:comment "A .torrent file which contains references(ndo:TorrentedFile) to files available via BitTorrent. The references are pointed to via nie:hasLogicalPart" ;
    rdfs:label "torrent" ;
    rdfs:subClassOf nie:InformationElement .

ndo:TorrentedFile
    a rdfs:Class ;
    rdfs:comment "A file available via a BitTorrent peer-to-peer network" ;
    rdfs:label "torrented file" ;
    rdfs:subClassOf ndo:P2PFile .

ndo:copiedFrom
    a rdf:Property ;
    rdfs:comment "Links a DataObject with its copy. This relation means that originally the Data Objects were copies but might have changed subsequentially." ;
    rdfs:domain nie:DataObject ;
    rdfs:label "copied from" ;
    rdfs:range nie:DataObject .

ndo:referrer
    a rdf:Property ;
    rdfs:comment "Points to the Information Element that contained the link to the download source which was used in the download event." ;
    rdfs:domain ndo:DownloadEvent ;
    rdfs:label "referrer" ;
    rdfs:range nie:InformationElement .

<http://www.semanticdesktop.org/ontologies/2010/04/30/ndo/metadata>
    nao:serializationLanguage "TriG" ;
    nrl:coreGraphMetadataFor <http://www.semanticdesktop.org/ontologies/2010/04/30/ndo#> ;
    a nrl:DocumentGraph, nrl:GraphMetadata .

