@prefix rdf: <http://www.w3.org/1999/02/22-rdf-syntax-ns#> .
@prefix rdfs: <http://www.w3.org/2000/01/rdf-schema#> .
@prefix nao: <http://www.semanticdesktop.org/ontologies/2007/08/15/nao#> .
@prefix nrl: <http://www.semanticdesktop.org/ontologies/2007/08/15/nrl#> .
@prefix xsd: <http://www.w3.org/2001/XMLSchema#> .

<http://www.semanticdesktop.org/ontologies/2007/08/15/nrl#>
    nao:description "NRL was designed for knowledge representation in Nepomuk Social Semantic Desktop applications. While being built on top of the Resource Description Framework (RDF) and the associated RDF Schema (RDFS), it addresses several limitations of current Semantic Web languages, especially with respect to modularization and costumization. These questions seem to be important not only in Semantic Desktop scenarios but also on the general Semantic Web. NRL tackles these questions by including support for two main additional concepts: Named Graphs and Graph Views. Named graphs help coping with the heterogeneity of knowledge models and ontologies, esp. multiple knowledge modules with potentially different interpretations. The view concept allows for the tailoring of ontologies towards different needs in various exploiting applications. This view concept provides also the basic mechanism to impose different semantics on thesame syntactical structure." ;
    nao:hasDefaultNamespace "http://www.semanticdesktop.org/ontologies/2007/08/15/nrl#" ;
    nao:hasDefaultNamespaceAbbreviation "nrl" ;
    nao:lastModified "2011-12-13T12:02:32.866Z" ;
    nao:prefLabel "Nepomuk Representation Language" ;
    nao:serializationLanguage "TriG" ;
    nao:status "Testing" ;
    nao:version "${SHAREDDESKTOPONTOLOGIES_VERSION}" ;
    nrl:updatable "0" ;
    a nrl:DocumentGraph, nrl:KnowledgeBase .

nrl:AsymmetricProperty
    a rdfs:Class ;
    rdfs:comment "A marker class to identify asymmetric properties" ;
    rdfs:label "AsymmetricProperty" ;
    rdfs:subClassOf rdfs:Resource .

nrl:Configuration
    a rdfs:Class ;
    rdfs:comment "Represents a named graph containing configuration data" ;
    rdfs:label "Configuration" ;
    rdfs:subClassOf nrl:Data .

nrl:Data
    a rdfs:Class ;
    rdfs:comment "An abstract class representing all named graph roles" ;
    rdfs:label "Data" ;
    rdfs:subClassOf nrl:Graph .

nrl:DefaultGraph
    a nrl:Graph ;
    rdfs:comment "Represents the default graph, the graph which contains any triple that does not belong to any other named graph" ;
    rdfs:label "DefaultGraph" .

nrl:DefiningProperty
    a rdfs:Class ;
    rdfs:comment """A defining property's value is part of what defines a resource, changing it means
                          means chaning the identity of the resource. The set of values of all defining
                          properties of a resource make up its identify.
                          Whenever comparing resources or sharing them the value of this property should
                          be taken into account. By default all properties with a literal range are to be
                          treated as defining properties unless they are marked as nrl:NonDefiningProperty.""" ;
    rdfs:label "defining property" ;
    rdfs:subClassOf rdf:Property .

nrl:DiscardableInstanceBase
    a rdfs:Class ;
    rdfs:comment "A named graph containing instance data that can be recreated by analyzing the original resources. Intended to be used by metadata extractors." ;
    rdfs:label "DiscardableInstanceBase" ;
    rdfs:subClassOf nrl:InstanceBase .

nrl:DocumentGraph
    a rdfs:Class ;
    rdfs:comment "A marker class to identify named graphs that exist within a physical document" ;
    rdfs:label "DocumentGraph" ;
    rdfs:subClassOf nrl:Graph .

nrl:ExternalViewSpecification
    a rdfs:Class ;
    rdfs:comment "Represents an external view specification, this usually being a program which automatically generates the required view for an input graph" ;
    rdfs:label "ExternalViewSpecification" ;
    rdfs:subClassOf nrl:ViewSpecification .

nrl:FunctionalProperty
    a rdfs:Class ;
    rdfs:comment "A marker class to identify functional properties" ;
    rdfs:label "FunctionalProperty" ;
    rdfs:subClassOf rdfs:Resource .

nrl:Graph
    a rdfs:Class ;
    rdfs:comment "Represents a named graph" ;
    rdfs:label "Graph" ;
    rdfs:subClassOf rdfs:Resource .

nrl:GraphMetadata
    a rdfs:Class ;
    rdfs:comment "Represents a special named graph that contains metadata for another graph" ;
    rdfs:label "GraphMetadata" ;
    rdfs:subClassOf nrl:Data .

nrl:GraphView
    a rdfs:Class ;
    rdfs:comment "Identifies a graph which is itself a view of another named graph" ;
    rdfs:label "GraphView" ;
    rdfs:subClassOf nrl:Graph .

nrl:InstanceBase
    a rdfs:Class ;
    rdfs:comment "Represents a named graph containing instance data" ;
    rdfs:label "InstanceBase" ;
    rdfs:subClassOf nrl:Data .

nrl:InverseFunctionalProperty
    a rdfs:Class ;
    rdfs:comment "A marker class to identify inverse functional properties" ;
    rdfs:label "InverseFunctionalProperty" ;
    rdfs:subClassOf rdfs:Resource .

nrl:KnowledgeBase
    a rdfs:Class ;
    rdfs:comment "Represents a named graph containing both schematic and instance data" ;
    rdfs:label "KnowledgeBase" ;
    rdfs:subClassOf nrl:InstanceBase, nrl:Ontology .

nrl:NonDefiningProperty
    a rdfs:Class ;
    rdfs:comment """A non-defining property's value is not part of what defines a resource, it rather
                          is part of the resource's state or expresses an opinion about the resource. Whenever
                          comparing resources or sharing them the value of this property should not be taken into
                          account. By default all properties with a resource range are to be treated as
                          non-defining properties unless they are marked as nrl:DefiningProperty.""" ;
    rdfs:label "non-defining property" ;
    rdfs:subClassOf rdf:Property .

nrl:Ontology
    a rdfs:Class ;
    rdfs:comment "Represents a named graph having the role of an Ontology" ;
    rdfs:label "Ontology" ;
    rdfs:subClassOf nrl:Schema .

nrl:ReflexiveProperty
    a rdfs:Class ;
    rdfs:comment "A marker class to identify reflexive properties" ;
    rdfs:label "ReflexiveProperty" ;
    rdfs:subClassOf rdfs:Resource .

nrl:RuleViewSpecification
    a rdfs:Class ;
    rdfs:comment "Represents a view specification that is composed of a set of rules which generate the required view from the input graph upon firing" ;
    rdfs:label "RuleViewSpecification" ;
    rdfs:subClassOf nrl:ViewSpecification .

nrl:Schema
    a rdfs:Class ;
    rdfs:comment "Represents a named graph containing schematic data" ;
    rdfs:label "Schema" ;
    rdfs:subClassOf nrl:Data .

nrl:Semantics
    a rdfs:Class ;
    rdfs:comment "Represents some declarative semantics" ;
    rdfs:label "Semantics" ;
    rdfs:subClassOf rdfs:Resource .

nrl:SymmetricProperty
    a rdfs:Class ;
    rdfs:comment "A marker class to identify symmetric properties" ;
    rdfs:label "SymmetricProperty" ;
    rdfs:subClassOf rdfs:Resource .

nrl:TransitiveProperty
    a rdfs:Class ;
    rdfs:comment "A marker class to identify transitive properties" ;
    rdfs:label "TransitiveProperty" ;
    rdfs:subClassOf rdfs:Resource .

nrl:ViewSpecification
    a rdfs:Class ;
    rdfs:comment "Represents a specification of the means to achieve a transformation of an input graph into the required graph view" ;
    rdfs:label "ViewSpecification" ;
    rdfs:subClassOf rdfs:Resource .

nrl:cardinality
    a rdf:Property ;
    rdfs:comment "Specifies the precise value cardinality for a specific property" ;
    rdfs:domain rdf:Property ;
    rdfs:label "cardinality" ;
    rdfs:range rdfs:Literal .

nrl:coreGraphMetadataFor
    a nrl:InverseFunctionalProperty, rdf:Property ;
    rdfs:comment "Links a metadata graph to the graph for which it specifies the core graph properties including the semantics and the graph namespace. A graph can have only one unique core metadata graph" ;
    rdfs:domain nrl:GraphMetadata ;
    rdfs:label "coreGraphMetadataFor" ;
    rdfs:range nrl:Graph ;
    rdfs:subPropertyOf nrl:graphMetadataFor .

nrl:equivalentGraph
    a nrl:SymmetricProperty, rdf:Property ;
    rdfs:comment "Links two equivalent named graphs. A symmetric property" ;
    rdfs:domain nrl:Graph ;
    rdfs:label "equivalentGraph" ;
    rdfs:range nrl:Graph .

nrl:externalRealizer
    a rdf:Property ;
    rdfs:comment "Points to the location of the realizer for the external view specification" ;
    rdfs:domain nrl:ExternalViewSpecification ;
    rdfs:label "externalRealizer" ;
    rdfs:range rdfs:Literal .

nrl:graphMetadataFor
    nrl:minCardinality "1"^^xsd:nonNegativeInteger ;
    a rdf:Property ;
    rdfs:comment "Links a metadata graph to the graph that is being described. A unique value is compulsory" ;
    rdfs:domain nrl:GraphMetadata ;
    rdfs:label "graphMetadataFor" ;
    rdfs:range nrl:Graph .

nrl:hasSemantics
    a rdf:Property ;
    rdfs:comment "Points to a representation of the declarative semantics for a graph role" ;
    rdfs:domain nrl:Data ;
    rdfs:label "hasSemantics" ;
    rdfs:range nrl:Semantics .

nrl:hasSpecification
    a rdf:Property ;
    rdfs:comment "Points to the representation of the view specification required to generate the graph view in question" ;
    rdfs:domain nrl:GraphView ;
    rdfs:label "hasSpecification" ;
    rdfs:range nrl:ViewSpecification .

nrl:imports
    a rdf:Property ;
    rdfs:comment "Models a subsumption relationship between two graphs, stating that the object graph is imported and included in the subject graph" ;
    rdfs:domain nrl:Data ;
    rdfs:label "imports" ;
    rdfs:range nrl:Data ;
    rdfs:subPropertyOf nrl:superGraphOf .

nrl:inverseProperty
    a rdf:Property ;
    rdfs:comment "Links two properties and specifies their inverse behaviour" ;
    rdfs:domain rdf:Property ;
    rdfs:label "inverseProperty" ;
    rdfs:range rdf:Property .

nrl:maxCardinality
    a rdf:Property ;
    rdfs:comment "Specifies a maximum value cardinality for a specific property" ;
    rdfs:domain rdf:Property ;
    rdfs:label "maxCardinality" ;
    rdfs:range rdfs:Literal .

nrl:minCardinality
    a rdf:Property ;
    rdfs:comment "Specifies a minimum value cardinality for a specific property" ;
    rdfs:domain rdf:Property ;
    rdfs:label "minCardinality" ;
    rdfs:range rdfs:Literal .

nrl:realizes
    a rdf:Property ;
    rdfs:comment "Points to a representation of the declarative semantics that the view specification realizes" ;
    rdfs:domain nrl:ViewSpecification ;
    rdfs:label "realizes" ;
    rdfs:range nrl:Semantics .

nrl:rule
    a rdf:Property ;
    rdfs:comment "Specifies rules for a view specification that is driven by rules" ;
    rdfs:domain nrl:RuleViewSpecification ;
    rdfs:label "rule" ;
    rdfs:range rdfs:Literal .

nrl:ruleLanguage
    a rdf:Property ;
    rdfs:comment "Specifies the rule language for a view specification that is driven by rules" ;
    rdfs:domain nrl:RuleViewSpecification ;
    rdfs:label "ruleLanguage" ;
    rdfs:range rdfs:Literal .

nrl:semanticsDefinedBy
    a rdf:Property ;
    rdfs:comment "Points to the human readable specifications for a representation of some declarative semantics" ;
    rdfs:domain nrl:Semantics ;
    rdfs:label "semanticsDefinedBy" ;
    rdfs:range rdfs:Resource .

nrl:subGraphOf
    nrl:inverseProperty nrl:superGraphOf ;
    a rdf:Property ;
    rdfs:comment "Specifies a containment relationship between two graphs, meaning that the subject graph is included in the object graph" ;
    rdfs:domain nrl:Graph ;
    rdfs:label "subGraphOf" ;
    rdfs:range nrl:Graph .

nrl:superGraphOf
    nrl:inverseProperty nrl:subGraphOf ;
    a rdf:Property ;
    rdfs:comment "Specifies a subsumption relationship between two graphs, meaning that the object graph is included in the subject graph" ;
    rdfs:domain nrl:Graph ;
    rdfs:label "superGraphOf" ;
    rdfs:range nrl:Graph .

nrl:updatable
    nrl:maxCardinality "1"^^xsd:nonNegativeInteger ;
    a rdf:Property ;
    rdfs:comment "A core graph metadata property, this defines whether a graph can be freely updated '1' or otherwise '0'" ;
    rdfs:domain nrl:Graph ;
    rdfs:label "updatable" ;
    rdfs:range xsd:boolean .

nrl:viewOn
    a rdf:Property ;
    rdfs:comment "Points to a graph view over the subject named graph" ;
    rdfs:domain nrl:GraphView ;
    rdfs:label "viewOn" ;
    rdfs:range nrl:Graph .

<http://www.semanticdesktop.org/ontologies/2007/08/15/nrl/metadata>
    nao:serializationLanguage "TriG" ;
    nrl:coreGraphMetadataFor <http://www.semanticdesktop.org/ontologies/2007/08/15/nrl#> ;
    a nrl:DocumentGraph, nrl:GraphMetadata .

